Hacl.operations: helper function to set all bytes of a buffer

crypto_hst/utils/Hacl.Operations.Pure.fst
@@ -8,6 +8,7 @@ open FStar.UInt32
 
 
 (* Define base types *)
+let u8 = FStar.UInt8.t
 let u32 = FStar.UInt32.t
 let s32 = Hacl.UInt32.t
 let bytes = Seq.seq Hacl.UInt8.t
@@ -21,3 +22,6 @@ let rotate_right (a:s32) (b:u32{v b <= 32}) : Tot s32 =
 (* Define helper xor function *)
 assume val xor_bytes: a:bytes -> b:bytes -> len:u32{v len <= Seq.length a /\ v len <= Seq.length b} 
   -> Tot (output:bytes{Seq.length output = v len})
+
+
+assume val setall: (b:bytes) -> (l:u32{Seq.length b = v l}) -> (x:u8) -> Tot (bf:bytes)
